Implementation/Lean/Cpn2mCrl2.lean
@@ -1,6 +1,7 @@
 import Cpn2mCrl2.Util
 import Cpn2mCrl2.Color
 import Cpn2mCrl2.Bag
+import Cpn2mCrl2.ListOps
 import Cpn2mCrl2.Expr
 import Cpn2mCrl2.Typing
 import Cpn2mCrl2.Net
